## Exercise 1

Use a direct proof to show that the sum of two odd integers is even.

In order to prove that the sum of two odd numbers is even we will use a direct proof. Let imagine we have two odd numbers a and b which have the form 2k + 1.
Therefore:
(2t+1) + (2i+1) = 2y
2t+2k = 2y-2
2(t+k) = 2(y-2)

Since both of the side of the equation have the form 2k+1, we can conclude that the sum of odd number is always even.

**PERFECT** (?)

Can be proven as well with a+ b = (2s + 1) + (2t + 1) = 2(s + t + 1)

## Exercise 3

Show that the square of an even number is an even number using a direct proof.

Let say that a is an even number. We know that an even number can be noted 2k. Therefore:
2k ^2 = 4k ^ 2 = 2(2k^2)
Since 2(2k^2) if of form 2k, the result of the square of an even number is an even number.

**PERFECT**


