## Exercise 17

Show that ¬(p ↔ q) and p ↔ ¬q are logically equivalent.

A biconditional statement is false if one of its operand is false. Hence  p ↔ q is equivalent to ¬p ↔ q and to p ↔ ¬q.

**PERFECT**

## Exercise 29

Show that (p → q) ∧ (q → r) → (p → r) is a tautol-
ogy.

Let's assume thant (p → q) ∧ (q → r) → (p → r) is not a tautology, hence the proposition can be false.
((p → q) ∧ (q → r)) → ((p → r)) to be false (p → q) ∧ (q → r) need to be true AND (p → r) needs to be false.
For (p → r) to be false we need r to be false and p to be true. We can modify the first part of the proposition as follow:(T → q) ∧ (q → F).
For (T → q) ∧ (q → F) to be true we need both (T → q) AND (q → F) to be true.
For (T → q) to be true we need q to be true and for (q → F) to be true we need q to be false.
q can't be true and false at the same time. This is a contradiction therefore (p → q) ∧ (q → r) → (p → r) cannot be false and is a tautology.

**PERFECT**

## Exercise 31

Show that (p → q) → r and p → (q → r) are not logically equivalent.

To find that the proposition is not logically equivalent we need to find value for p, q and r such as the truth values of (p → q) → r and p → (q → r) differ.
If p is false, q is false and r is false, hence (F → F) → F is equivalent to T → F and is false. However F → (F → F) is equivalent to F → T and is true.
Therefore (p → q) → r and p → (q → r) are not logically equivalent.

**PERFECT**

## Exercise 35

Find the dual of each of these compound propositions.
a) p ∧ ¬q ∧ ¬r 
b) (p ∧ q ∧ r) ∨ s
c) (p ∨ F) ∧ (q ∨ T)

a) p ∨ ¬q ∨ ¬r 
b) (p ∨ q ∨ r) ∧ s
c) (p ∧ T) ∨ (q ∧ F)

**PERFECT**
