# Exercise 1

1. Find f(1), f(2), f(3), and f(4) if f(n) is defined recursively by f(0) = 1 and for n = 0, 1, 2, . . .

a) f (n + 1) = f(n) + 2.
b) f (n + 1) = 3f(n).
c) f (n + 1) = 2^f(n).
d) f (n + 1) = f(n)^2 + f(n) + 1.

a) f(0) = 1
   f(1) = 1 + 2 = 3
   f(2) = 3 + 2 = 5
   f(3) = 5 + 2 = 7
   f(4) = 7 + 2 = 9

b) f(0) = 1
   f(1) = 3 * 1 = 3
   f(2) = 3 * 3 = 9
   f(3) = 3 * 9 = 27
   f(4) = 3 * 27 = 81

c) f(0) = 1
   f(1) = 2^1 = 2
   f(2) = 2^2 = 4
   f(3) = 2^4 = 16
   f(4) = 2^16 = 65536

d) f(0) = 1
   f(1) = 1^2 + 1 + 1 = 3
   f(2) = 3^2 + 3 + 1 = 13
   f(3) = 13^2 + 13 + 1 = 183
   f(4) = 183^2 + 183 + 1 = 33673
